#代数 #环论 #组合数学 

>[!theorem] 二项式定理 (Binomial Theorem)
>设$R$是[[环]], 对于$a,b\in R, n\in\N$, 若$ab=ba$, 则有
>$${(a+b)}^n=\sum_{k=0}^{n}{\binom{n}{k}a^{n-k}b^k}$$

>[!proof]
>用数学归纳法, 先证基例: 显然${(a+b)}^0=\binom{0}{0}a^0b^0=1$成立.
>接下来证明${(a+b)}^{m-1}=\sum_{k=0}^{m-1}{\binom{m-1}{k}a^{m-k-1}b^k}$能推出${(a+b)}^m=\sum_{k=0}^{m}{\binom{m}{k}a^{m-k}b^k}$, 显然有
>$$\begin{aligned}{(a+b)}^m&={(a+b)}^{m-1}(a+b)=(a+b)\sum_{k=0}^{m-1}{\binom{m-1}{k}a^{m-k-1}b^k}\\&=\sum_{k=0}^{m-1}{\binom{m-1}{k}a^{m-k}b^k} + \sum_{k=0}^{m-1}{\binom{m-1}{k}a^{m-k-1}b^{k+1}} \\&=\sum_{k=0}^{m-1}{\binom{m-1}{k}a^{m-k}b^k} + \sum_{k=1}^{m}{\binom{m-1}{k-1}a^{m-k}b^{k}} \\&=\binom{m-1}{0}a^{m} + \sum_{k=1}^{m-1}\left[\binom{m-1}{k}+\binom{m-1}{k-1}\right]a^{m-k}b^{k} + \binom{m-1}{m-1}b^{m} \\&=a^{m} + \sum_{k=1}^{m-1}\binom{m}{k}a^{m-k}b^{k} + b^{m} \\&=\sum_{k=0}^{m}{\binom{m}{k}a^{m-k}b^{k}}\end{aligned}$$
>这就证明了原定理.
